add rank stuff to address decreases in Linked

Splinter/Betree/LinkedBetreeRefinement.i.dfy
@@ -16,9 +16,14 @@ module LinkedBetreeRefinement {
   import opened StampedMod
   import PivotBetree
 
-  function EmptyStampedBetree() : StampedBetree
+  function EmptyStampedBetree() : (out: StampedBetree)
+    ensures Acyclic(out.value.diskView)
   {
-    Stamped(LinkedBetree(None, DiskView(map[])), 0)
+    var out := Stamped(LinkedBetree(None, DiskView(map[])), 0);
+    assert Acyclic(out.value.diskView) by {
+      assert PointersRespectRank(out.value.diskView, map[]);
+    }
+    out
   }
 
   function ILbl(lbl: TransitionLabel) : PivotBetree.TransitionLabel
@@ -28,16 +33,51 @@ module LinkedBetreeRefinement {
       case PutLabel(puts) => PivotBetree.PutLabel(puts)
       case QueryEndLsnLabel(endLsn) => PivotBetree.QueryEndLsnLabel(endLsn)
       case FreezeAsLabel(stampedBetree) => PivotBetree.FreezeAsLabel(
-        if stampedBetree.value.WF()
+        if stampedBetree.value.WF() && Acyclic(stampedBetree.value.diskView)
         then IStampedBetree(stampedBetree)
-        else IStampedBetree(EmptyStampedBetree())
+        else IStampedBetree(EmptyStampedBetree())  // "silly" case, since we never interpret non-(WF+Acyclic) things
       )
       case InternalLabel() => PivotBetree.InternalLabel()
+  }
+
+  predicate PointersRespectRank(diskView: DiskView, ranking: GenericDisk.Ranking)
+    requires diskView.WF()
+  {
+    && diskView.entries.Keys <= ranking.Keys
+    && (forall address | address in diskView.entries
+        :: var node := diskView.entries[address];
+          forall childIdx:nat | node.ValidChildIndex(childIdx) && node.children[childIdx].Some?
+            :: ranking[node.children[childIdx].value] < ranking[address]
+        )
+  }
+
+  predicate Acyclic(diskView: DiskView)
+  {
+    && diskView.WF()
+    && (exists ranking :: PointersRespectRank(diskView, ranking))
+  }
+
+  function TheRanking(diskView: DiskView) : GenericDisk.Ranking
+    requires diskView.WF()
+    requires Acyclic(diskView)
+  {
+    // Make CHOOSE deterministic as Leslie and Hilbert intended
+    var ranking :| PointersRespectRank(diskView, ranking); ranking
+  }
+
+  function TheRankOf(linked: LinkedBetree) : int
+    requires linked.WF()
+  {
+    if linked.HasRoot() && Acyclic(linked.diskView) then TheRanking(linked.diskView)[linked.root.value] else -1
+    // Rustan: I can't believe this works! How are you figuring out that we can pass 0 into
+    // negatives, but we stop there!?
   }
 
   function IChildren(linked: LinkedBetree) : seq<PivotBetree.BetreeNode>
     requires linked.WF()
     requires linked.HasRoot()
+    requires Acyclic(linked.diskView)
+    decreases TheRankOf(linked), 0
   {
     var numChildren := |linked.Root().children|;
     seq(numChildren, i requires 0<=i<numChildren => ILinkedBetree(linked.ChildAtIdx(i)))
@@ -45,6 +85,8 @@ module LinkedBetreeRefinement {
 
   function ILinkedBetree(linked: LinkedBetree) : PivotBetree.BetreeNode
     requires linked.WF()
+    requires Acyclic(linked.diskView)
+    decreases TheRankOf(linked), 1
   {
     if linked.root.None?
     then PivotBetree.Nil
@@ -55,32 +97,38 @@ module LinkedBetreeRefinement {
 
   function IStampedBetree(stampedBetree: StampedBetree) : PivotBetree.StampedBetree
     requires stampedBetree.value.WF()
+    requires Acyclic(stampedBetree.value.diskView)
   {
     Stamped(ILinkedBetree(stampedBetree.value), stampedBetree.seqEnd)
   }
 
   function I(v: Variables) : PivotBetree.Variables
     requires v.WF()
+    requires Acyclic(v.linked.diskView)
   {
     PivotBetree.Variables(v.memtable, ILinkedBetree(v.linked))
   }
 
   predicate Inv(v: Variables)
   {
-    true  // TODO!
+    && Acyclic(v.linked.diskView)
   }
 
   lemma InitRefines(v: Variables, stampedBetree: StampedBetree)
     requires Init(v, stampedBetree)
+    ensures Inv(v)
     ensures PivotBetree.Init(I(v), IStampedBetree(stampedBetree))
   {
+    assume false;
   }
 
   lemma NextRefines(v: Variables, v': Variables, lbl: TransitionLabel)
     requires Inv(v)
     requires Next(v, v', lbl)
     ensures v'.WF()
+    ensures Inv(v')
     ensures PivotBetree.Next(I(v), I(v'), ILbl(lbl))
   {
+    assume false;
   }
 }
